FiatFormal/Language/Progress.v
@@ -8,78 +8,145 @@ Theorem fiatProgress
     TYPE alg_ds adt_ds nil x t
     -> value x \/ (exists x', STEP adt_ds x x') \/ Xhas_choice adt_ds x.
 Proof.
-(*  intros. gen t. *)
-(*  induction x using exp_mutind with *)
-(*      (PA := fun a => a = a) *)
-(*      (PF := fun f => f = f); rip; burn. *)
+ intros. gen t.
+ induction x using exp_mutind with
+     (PA := fun a => a = a)
+     (PF := fun f => f = f); rip; burn.
 
-(*  Case "XApp". *)
-(*   right; left. *)
-(*   inverts_type. *)
-(*   edestruct IHx1; eauto. *)
-(*   SCase "value x1". *)
-(*    edestruct IHx2; eauto. *)
-(*    SSCase "value x2". *)
+ Case "XApp".
+ right.
+ inverts_type.
+ edestruct IHx1; eauto.
 
-(*    (* next statement fails because XLam is not unique in the type (TFun _ _) *) *)
-(*     have HF: (exists t x, x1 = XLam t x). *)
-(*      destruct HF as [t11]. *)
-(*      destruct H1 as [x12]. *)
-(*      subst. *)
-(*      exists (substX 0 x2 x12). *)
-(*      eauto. *)
-(*     SSCase "x2 steps". *)
-(*      destruct H0 as [x2']. *)
-(*      exists (XApp x1 x2'). auto. *)
-(*   SCase "x1 steps". *)
-(*    destruct H  as [x1']. *)
-(*    exists (XApp x1' x2). *)
-(*    eapply (EsContext (fun xx => XApp xx x2)); auto. *)
+ SCase "value x1".
+ edestruct IHx2; eauto.
 
-(*  Case "XCon". *)
-(*   inverts_type. *)
+ SSCase "value x2".
+ assert (HF: exists t1 t2 x, x1 = XFix t1 t2 x).
+ { apply (value_fix _ _ _ _ _ _ H H5). }
+ destruct HF as [t11].
+ destruct H1 as [t12].
+ destruct H1 as [x12].
+ subst.
+ left.
+ exists (substX 0 (XFix t11 t12 x12) (substX 0 x2 x12)).
+ eauto.
+ destruct H0 as [[x2'] | HC].
 
-(*   (* All ctor args are either wnf or can step *) *)
-(*   assert (Forall (fun x => wnfX x \/ (exists x', STEP x x')) xs) as HWS. *)
-(*    norm. rip. *)
-(*    have (exists t, TYPE ds nil x t). dest t. *)
-(*    have (value x \/ (exists x', STEP x x')). *)
-(*    inverts H2; burn. *)
+ SSCase "x2 steps".
+ left.
+ exists (XApp x1 x2'). auto.
 
-(*   (* All ctor args are wnf, or there is a context where one can step *) *)
-(*   lets D: (@exps_ctx_run exp exp) HWS. *)
-(*   inverts D. *)
-(*    (* All ctor args are wnf *) *)
-(*    left. eauto 6. *)
-(*    (* There is a context where one ctor arg can step *) *)
-(*    right. *)
-(*     dest C. dest x'. *)
-(*     rip. *)
-(*     lets D: step_context_XCon_exists H1 H5. *)
-(*     destruct D as [x'']. eauto. *)
+ SSCase "x2 hasChoice".
+ right. eauto.
+ destruct H  as [[x1'] | HC].
 
-(*  Case "XCase". *)
-(*   right. *)
-(*   inverts_type. *)
-(*   have HS: (value x \/ (exists x', STEP x x')). *)
-(*   inverts HS. clear IHx. *)
-(*   SCase "x value". *)
-(*    destruct x; nope. *)
-(*     SSCase "XCon". *)
-(*      inverts_type. *)
-(*      rrwrite (dcs0 = dcs). *)
-(*      have HG: (exists ts x, getAlt d aa = Some (AAlt d ts x)) *)
-(*       by burn using getAlt_exists. *)
-(*      dest ts. dest x. *)
-(*      exists (substXs 0 l x). *)
-(*      burn. *)
+ SCase "x1 steps".
+ left.
+ exists (XApp x1' x2).
+ eapply (EsContext _ (fun xx => XApp xx x2)); auto.
 
-(*   SCase "x steps". *)
-(*    destruct H0 as [x']. *)
-(*    exists (XCase x' aa). *)
-(*    lets D: EsContext XcCase; eauto. *)
-(* Qed. *)
-Admitted.
+ SCase "x1 hasChoice".
+ right. eauto.
+
+
+ Case "XCon".
+  inverts_type.
+
+  (* All ctor args are either wnf or can step *)
+  assert (Forall (fun x => wnfX x \/ (exists x', STEP adt_ds x x') \/ (Xhas_choice adt_ds x)) xs) as HWS.
+   norm. rip.
+   have (exists t, TYPE alg_ds adt_ds nil x t). dest t.
+   have (value x \/ (exists x', STEP adt_ds x x') \/ (Xhas_choice adt_ds x)).
+   inverts H2; burn.
+
+  (* All ctor args are wnf, or there is a context where one can step *)
+  lets D: (@exps_ctx_run exp exp) HWS.
+  inverts D.
+   (* All ctor args are wnf *)
+   left. eauto 6.
+   (* There is a context where one ctor arg can step *)
+   right.
+    dest C. dest x'.
+    rip.
+    inverts H5.
+    left.
+    lets D: step_context_XCon_exists H1 H0.
+    destruct D as [x'']. eauto.
+    right.
+    apply HC_XCon. apply Exists_exists.
+    exists x'; rip.
+    eapply exps_In_C_pmk. eassumption.
+
+ Case "XMatch".
+  right.
+  inverts_type.
+  have HS: (value x \/ (exists x', STEP adt_ds x x') \/ (Xhas_choice adt_ds x)).
+  inverts HS. clear IHx.
+  SCase "x value".
+   destruct x; nope.
+    SSCase "XCon".
+     inverts_type.
+     rrwrite (dcs0 = dcs).
+     have HG: (exists ts x, getAlt d aa = Some (AAlt d ts x))
+      by burn using getAlt_exists.
+     dest ts. dest x.
+     left.
+     exists (substXs 0 l x).
+     burn.
+
+  SCase "x steps or hasChoice".
+  destruct H0 as [[x'] | HC].
+  left.
+  exists (XMatch x' aa).
+  lets D: EsContext XcMatch; eauto.
+  SSCase "x hasChoice".
+  right.
+  eauto.
+
+  Case "XCall".
+
+  pose proof (wellTypedCallHasBody_pmk _ _ _ _ _ _ _ H0).
+  inverts_type.
+  (* pose proof (Forall2_Forall_left _ _ _ _ H H11). *)
+
+  assert (Forall (fun x => wnfX x \/ (exists x', STEP adt_ds x x') \/ (Xhas_choice adt_ds x)) xs) as HWS.
+  norm. rip.
+   have (exists t, TYPE alg_ds adt_ds nil x t). dest t.
+   have (value x \/ (exists x', STEP adt_ds x x') \/ (Xhas_choice adt_ds x)).
+   inverts H4; burn.
+
+  (* All method args are wnf, or there is a context where one can step *)
+  (*    or haschoice *)
+  lets D: (@exps_ctx_run exp exp) HWS.
+  right.
+  inverts D.
+  SCase "xs all wnf".
+
+  (* All method args are wnf, must show a step with method body *)
+  (* rewrite Forall_forall in H0. *)
+  (* spec H0 ac. *)
+  (* pose proof (getADTSigInCons_pmk _ _ _ _ H10). *)
+  (* spec H0 H4. invert H0; intros. *)
+
+  dest b. left.
+  exists (substXs 0 xs b).
+  apply EsADTCall; burn.
+
+   (* There is a context where one ctor arg can step *)
+    dest C. dest x'.
+    rip.
+    inverts H5.
+    left.
+    lets D: step_context_XCall_exists_pmk H3 H2.
+    destruct D as [x'']. eauto.
+    right.
+    apply HC_XCallArgs. apply Exists_exists.
+    exists x'; rip.
+    eapply exps_In_C_pmk. eassumption.
+
+Qed.
+
 
 (* ORIG *)
 (* A well typed expression is either a well formed value,
